inv errors fixed

txn-data-consistency/CCv_Eiger_Port_plus.thy
@@ -12,12 +12,18 @@ type_synonym svr_id = key
 type_synonym tstmp = nat
 
 \<comment> \<open>Server State\<close>
-datatype 'v ver_state = Prep tstmp 'v | Commit tstmp 'v "txid0 set"
-type_synonym 'v state_wtxn = "txid \<rightharpoonup> 'v ver_state"
+datatype 'v ver_state = No_Ver | Prep tstmp 'v | Commit tstmp 'v "txid0 set"
+type_synonym 'v state_wtxn = "txid \<Rightarrow> 'v ver_state"
 record 'v server =
   wtxn_state :: "'v state_wtxn"
   clock :: tstmp
   lst :: tstmp
+
+definition wts_dom :: "'v state_wtxn \<Rightarrow> txid set" where
+  "wts_dom wts \<equiv> {t. wts t \<noteq> No_Ver}"
+
+abbreviation wts_emp :: "'v state_wtxn" where
+  "wts_emp \<equiv> (\<lambda>t. No_Ver)"
 
 \<comment> \<open>Client State\<close>
 datatype 'v state_txn =
@@ -41,7 +47,7 @@ record 'v state =
   cls :: "cl_id \<Rightarrow> 'v client"
   svrs :: "svr_id \<Rightarrow> 'v server"
   commit_order :: "key \<Rightarrow> txid list" \<comment> \<open>history variable - not used for the algorithm itself\<close>
-  (* inv: all txids in the list have committed versions for that key *)
+  (* inv: all txids in the list have committed/prepared versions for that key *)
 
 subsubsection \<open>Functions\<close>
 
@@ -61,14 +67,17 @@ fun get_sn_wtxn :: "txid \<Rightarrow> sqn" where
   "get_sn_wtxn (Tn (Tn_cl sn cl)) = sn"
 
 fun get_val_ver :: "'v ver_state \<Rightarrow> 'v" where
+  "get_val_ver No_Ver = undefined" |
   "get_val_ver (Prep _ v) = v" |
   "get_val_ver (Commit _ v _) = v"
 
 fun get_ts_ver :: "'v ver_state \<Rightarrow> tstmp" where
+  "get_ts_ver No_Ver = undefined" |
   "get_ts_ver (Prep ts _) = ts" |
   "get_ts_ver (Commit cts _ _) = cts"
 
 fun get_rs_ver :: "'v ver_state \<Rightarrow> txid0 set" where
+  "get_rs_ver No_Ver = undefined" |
   "get_rs_ver (Prep _ _) = {}" |
   "get_rs_ver (Commit _ _ rs) = rs"
 
@@ -77,29 +86,27 @@ fun get_rs_ver :: "'v ver_state \<Rightarrow> txid0 set" where
 
 \<comment> \<open>returns greatest commit timestamp (cts) less than read timestamp (rts)\<close>
 definition committed_at where
-  "committed_at wtxn_s t cts \<equiv> \<exists>v rs. wtxn_s t = Some (Commit cts v rs)"
+  "committed_at wts t cts \<equiv> \<exists>v rs. wts t = Commit cts v rs"
 
 definition at_cts :: "'v state_wtxn \<Rightarrow> tstmp \<Rightarrow> tstmp" where
-  "at_cts wtxn_s rts \<equiv> GREATEST cts. cts \<le> rts \<and> (\<exists>t. committed_at wtxn_s t cts)"
+  "at_cts wts rts \<equiv> GREATEST cts. cts \<le> rts \<and> (\<exists>t. committed_at wts t cts)"
 
 \<comment> \<open>(Probably redundant) returns the version read at read timestamp (highest cts less than ts)\<close>
 definition at :: "'v state_wtxn \<Rightarrow> tstmp \<Rightarrow> txid" where
-  "at wtxn_s rts \<equiv> SOME t. committed_at wtxn_s t (at_cts wtxn_s rts)"
-
-lemma "get_ts_ver (the (wtxn_s (at wtxn_s rts))) = at_cts wtxn_s rts" oops
+  "at wts rts \<equiv> SOME t. committed_at wts t (at_cts wts rts)"
 
 abbreviation has_newer_own_write :: "'v state_wtxn \<Rightarrow> tstmp \<Rightarrow> cl_id \<Rightarrow> bool" where
-  "has_newer_own_write wtxn_s cts cl \<equiv> \<exists>t. get_cl_wtxn t = cl \<and> committed_at wtxn_s t cts"
+  "has_newer_own_write wts cts cl \<equiv> \<exists>t. get_cl_wtxn t = cl \<and> committed_at wts t cts"
 
 definition newest_own_write :: "'v state_wtxn \<Rightarrow> tstmp \<Rightarrow> cl_id \<rightharpoonup> txid" where
-  "newest_own_write wtxn_s ts cl \<equiv>
-    (if (\<exists>cts. has_newer_own_write wtxn_s cts cl \<and> cts \<ge> ts)
-     then Some (SOME t. \<exists>v rs. wtxn_s t = Some (Commit (GREATEST cts. has_newer_own_write wtxn_s cts cl \<and> cts \<ge> ts) v rs))
+  "newest_own_write wts ts cl \<equiv>
+    (if (\<exists>cts. has_newer_own_write wts cts cl \<and> cts \<ge> ts)
+     then Some (SOME t. \<exists>v rs. wts t = Commit (GREATEST cts. has_newer_own_write wts cts cl \<and> cts \<ge> ts) v rs)
      else None)"
 
 definition read_at :: "'v state_wtxn \<Rightarrow> tstmp \<Rightarrow> cl_id \<Rightarrow> txid" where
-  "read_at wtxn_s ts cl \<equiv> let t = at wtxn_s ts in
-    (case newest_own_write wtxn_s (get_ts_ver (the (wtxn_s t))) cl of
+  "read_at wts ts cl \<equiv> let t = at wts ts in
+    (case newest_own_write wts (get_ts_ver (wts t)) cl of
       None \<Rightarrow> t |
       Some t' \<Rightarrow> t')"
 
@@ -107,26 +114,26 @@ definition read_at :: "'v state_wtxn \<Rightarrow> tstmp \<Rightarrow> cl_id \<R
 \<comment> \<open>Helper functions\<close>
 
 definition add_to_readerset :: "'v state_wtxn \<Rightarrow> txid0 \<Rightarrow> txid \<Rightarrow> 'v state_wtxn" where
-  "add_to_readerset wtxn_s t t_wr \<equiv> (case wtxn_s t_wr of
-    Some (Commit cts v rs) \<Rightarrow> wtxn_s (t_wr \<mapsto> Commit cts v (insert t rs)) |
-    _ \<Rightarrow> wtxn_s)"
+  "add_to_readerset wts t t_wr \<equiv> (case wts t_wr of
+    Commit cts v rs \<Rightarrow> wts (t_wr := Commit cts v (insert t rs)) |
+    _ \<Rightarrow> wts)"
 
-abbreviation view_txid_vid' :: "'v state \<Rightarrow> view_txid \<Rightarrow> view" where
-  "view_txid_vid' s u \<equiv> (\<lambda>k. (inv ((!) (commit_order s k))) ` (u k))"
+definition view_txid_vid :: "'v state \<Rightarrow> view_txid \<Rightarrow> view" where
+  "view_txid_vid s u \<equiv> (\<lambda>k. (inv ((!) (commit_order s k))) ` (u k))"
 
-abbreviation view_txid_vid :: "'v state \<Rightarrow> view_txid \<Rightarrow> view" where
-  "view_txid_vid s u \<equiv> (\<lambda>k. List.map_project (\<lambda>tid. if tid \<in> set (commit_order s k)
-    then Some (SOME i. (commit_order s k) ! i = tid) else None) (u k))"
+definition view_txid_vid' :: "'v state \<Rightarrow> view_txid \<Rightarrow> view" where
+  "view_txid_vid' s u \<equiv> (\<lambda>k. List.map_project (\<lambda>tid. if tid \<in> set (commit_order s k)
+    then Some (SOME i. i < length (commit_order s k) \<and> (commit_order s k) ! i = tid) else None) (u k))"
 
 (* inv: showing all elements of view exist in commit_order *)
 (* inv: commit_order distinct *)
 
 definition get_view :: "'v state \<Rightarrow> cl_id \<Rightarrow> view_txid" where
-  "get_view s cl \<equiv> (\<lambda>k. {t. \<exists>cts v rs. wtxn_state (svrs s k) t = Some (Commit cts v rs) \<and>
+  "get_view s cl \<equiv> (\<lambda>k. {t. \<exists>cts v rs. wtxn_state (svrs s k) t = Commit cts v rs \<and>
     (cts \<le> gst (cls s cl) \<or> get_cl_wtxn t = cl)})"
 
 definition pending_wtxns where
-  "pending_wtxns s k \<equiv> {prep_t. \<exists>t v. wtxn_state (svrs s k) t = Some (Prep prep_t v)}"
+  "pending_wtxns s k \<equiv> {prep_t. \<exists>t v. wtxn_state (svrs s k) t = Prep prep_t v}"
 
 
 subsubsection \<open>Events\<close>
@@ -139,18 +146,21 @@ datatype 'v ev =
 definition other_insts_unchanged where
   "other_insts_unchanged e s s' \<equiv> \<forall>e'. e' \<noteq> e \<longrightarrow> s' e' = s e'"
 
-definition cls_svr_k'_t'_unchanged where
-  "cls_svr_k'_t'_unchanged k s s' \<equiv> cls s' = cls s \<and> other_insts_unchanged k (svrs s) (svrs s')"
+definition cls_svr_k'_unchanged where
+  "cls_svr_k'_unchanged k s s' \<equiv> cls s' = cls s \<and> other_insts_unchanged k (svrs s) (svrs s')"
 
 definition svrs_cls_cl'_unchanged where
   "svrs_cls_cl'_unchanged cl s s' \<equiv> svrs s' = svrs s \<and> other_insts_unchanged cl (cls s) (cls s')"
 
-lemmas svr_unchanged_defs = cls_svr_k'_t'_unchanged_def other_insts_unchanged_def
+lemmas svr_unchanged_defs = cls_svr_k'_unchanged_def other_insts_unchanged_def
 lemmas cl_unchanged_defs = svrs_cls_cl'_unchanged_def other_insts_unchanged_def
 lemmas unchanged_defs = svr_unchanged_defs svrs_cls_cl'_unchanged_def
 
-definition tid_match :: "'v state \<Rightarrow> txid \<Rightarrow> bool" where
-  "tid_match s t \<equiv> txn_sn (cls s (get_cl_wtxn t)) = get_sn_wtxn t"
+definition tid_match :: "'v state \<Rightarrow> txid0 \<Rightarrow> bool" where
+  "tid_match s t \<equiv> txn_sn (cls s (get_cl_txn t)) = get_sn_txn t"
+
+definition wtid_match :: "'v state \<Rightarrow> txid \<Rightarrow> bool" where
+  "wtid_match s t \<equiv> txn_sn (cls s (get_cl_wtxn t)) = get_sn_wtxn t"
 
 \<comment> \<open>Clint Events\<close>
 definition read_invoke :: "cl_id \<Rightarrow> key set \<Rightarrow> 'v state \<Rightarrow> 'v state \<Rightarrow> bool" where
@@ -170,7 +180,7 @@ definition read :: "cl_id \<Rightarrow> key \<Rightarrow> 'v \<Rightarrow> txid 
   "read cl k v t s s' \<equiv> (\<exists>keys vals.
     txn_state (cls s cl) = RtxnInProg keys vals \<and> k \<in> keys \<and> vals k = None \<and>
     txn_state (cls s' cl) = RtxnInProg keys (vals (k \<mapsto> (v, t)))) \<and>
-    (\<exists>cts rs. wtxn_state (svrs s k) t = Some (Commit cts v rs) \<and> get_txn_cl s cl \<in> rs) \<and>
+    (\<exists>cts rs. wtxn_state (svrs s k) t = Commit cts v rs \<and> get_txn_cl s cl \<in> rs) \<and>
     txn_sn (cls s' cl) = txn_sn (cls s cl) \<and>
     gst (cls s' cl) = gst (cls s cl) \<and>
     lst_map (cls s' cl) = (lst_map (cls s cl)) (k := lst (svrs s k)) \<and>
@@ -213,9 +223,9 @@ definition write_commit :: "cl_id \<Rightarrow> (key \<rightharpoonup> 'v) \<Rig
     u'' = view_txid_vid s (get_view s cl) \<and>
     txn_state (cls s cl) = WtxnPrep kv_map \<and>
     (\<forall>k \<in> dom kv_map.
-      (\<exists>v prep_t. wtxn_state (svrs s k) (get_wtxn_cl s cl) = Some (Prep prep_t v))) \<and>
+      (\<exists>v prep_t. wtxn_state (svrs s k) (get_wtxn_cl s cl) = Prep prep_t v)) \<and>
     commit_t = Max {prep_t. (\<exists>k \<in> dom kv_map. \<exists>v.
-      wtxn_state (svrs s k) (get_wtxn_cl s cl) = Some (Prep prep_t v))} \<and>
+      wtxn_state (svrs s k) (get_wtxn_cl s cl) = Prep prep_t v)} \<and>
     txn_state (cls s' cl) = WtxnCommit commit_t kv_map \<and>
     txn_sn (cls s' cl) = txn_sn (cls s cl) \<and>
     gst (cls s' cl) = gst (cls s cl) \<and>
@@ -230,7 +240,7 @@ definition write_done :: "cl_id \<Rightarrow> 'v state \<Rightarrow> 'v state \<
   "write_done cl s s' \<equiv> 
     (\<exists>kv_map.
       (\<exists>commit_t. txn_state (cls s cl) = WtxnCommit commit_t kv_map \<and>
-        (\<forall>k\<in>dom kv_map. \<exists>v rs. wtxn_state (svrs s k) (get_wtxn_cl s cl) = Some (Commit commit_t v rs))) \<and>
+        (\<forall>k\<in>dom kv_map. \<exists>v rs. wtxn_state (svrs s k) (get_wtxn_cl s cl) = Commit commit_t v rs)) \<and>
       (\<forall>k \<in> dom kv_map. lst_map (cls s' cl) k = lst (svrs s k)) \<and>
       (\<forall>k. k \<notin> dom kv_map \<longrightarrow> lst_map (cls s' cl) k = lst_map (cls s cl) k) \<and>
       cl_clock (cls s' cl) = Suc (max (cl_clock (cls s cl)) (Max {clock (svrs s k) | k. k \<in> dom kv_map}))) \<and>
@@ -244,42 +254,42 @@ definition write_done :: "cl_id \<Rightarrow> 'v state \<Rightarrow> 'v state \<
 \<comment> \<open>Server Events\<close>
 definition register_read :: "svr_id \<Rightarrow> txid0 \<Rightarrow> 'v \<Rightarrow> txid \<Rightarrow> tstmp \<Rightarrow> 'v state \<Rightarrow> 'v state \<Rightarrow> bool" where
   "register_read svr t v t_wr gst_ts s s' \<equiv>
-    tid_match s (Tn t) \<and>
+    tid_match s t \<and>
     (\<exists>keys kvt_map.
       txn_state (cls s (get_cl_txn t)) = RtxnInProg keys kvt_map \<and> svr \<in> keys \<and> kvt_map svr = None) \<and>
     t_wr = read_at (wtxn_state (svrs s svr)) gst_ts (get_cl_txn t) \<and>
-    v = get_val_ver (the (wtxn_state (svrs s svr) t_wr)) \<and>
+    v = get_val_ver (wtxn_state (svrs s svr) t_wr) \<and>
     gst_ts = gst (cls s (get_cl_txn t)) \<and>
     wtxn_state (svrs s' svr) = add_to_readerset (wtxn_state (svrs s svr)) t t_wr \<and>
     clock (svrs s' svr) = Suc (max (clock (svrs s svr)) (cl_clock (cls s (get_cl_txn t)))) \<and>
     lst (svrs s' svr) = lst (svrs s svr) \<and>
-    cls_svr_k'_t'_unchanged svr s s' \<and>
+    cls_svr_k'_unchanged svr s s' \<and>
     commit_order s' = commit_order s"
 
 definition prepare_write :: "svr_id \<Rightarrow> txid \<Rightarrow> 'v \<Rightarrow> tstmp \<Rightarrow> 'v state \<Rightarrow> 'v state \<Rightarrow> bool" where
   "prepare_write svr t v gst_ts s s' \<equiv>
-    tid_match s t \<and>
+    wtid_match s t \<and>
     (\<exists>kv_map.
       txn_state (cls s (get_cl_wtxn t)) = WtxnPrep kv_map \<and> svr \<in> dom kv_map \<and> kv_map svr = Some v) \<and>
     gst_ts = gst (cls s (get_cl_wtxn t)) \<and>
-    wtxn_state (svrs s svr) t = None \<and>
-    wtxn_state (svrs s' svr) = wtxn_state (svrs s svr) (t \<mapsto> Prep (clock (svrs s svr)) v) \<and>
+    wtxn_state (svrs s svr) t = No_Ver \<and>
+    wtxn_state (svrs s' svr) = (wtxn_state (svrs s svr)) (t := Prep (clock (svrs s svr)) v) \<and>
     clock (svrs s' svr) = Suc (max (clock (svrs s svr)) (cl_clock (cls s (get_cl_wtxn t)))) \<and>
     lst (svrs s' svr) = lst (svrs s svr) \<and>
-    cls_svr_k'_t'_unchanged svr s s' \<and>
+    cls_svr_k'_unchanged svr s s' \<and>
     commit_order s' = commit_order s"
 
 definition commit_write :: "svr_id \<Rightarrow> txid \<Rightarrow> 'v state \<Rightarrow> 'v state \<Rightarrow> bool" where
   "commit_write svr t s s' \<equiv>
-    tid_match s t \<and>
+    wtid_match s t \<and>
     (\<exists>commit_t. (\<exists>kv_map. svr \<in> dom kv_map \<and>
       txn_state (cls s (get_cl_wtxn t)) = WtxnCommit commit_t kv_map) \<and>
-      (\<exists>prep_t v. wtxn_state (svrs s svr) t = Some (Prep prep_t v) \<and>
-        wtxn_state (svrs s' svr) = wtxn_state (svrs s svr) (t \<mapsto> Commit commit_t v {}))) \<and>
+      (\<exists>prep_t v. wtxn_state (svrs s svr) t = Prep prep_t v \<and>
+        wtxn_state (svrs s' svr) = (wtxn_state (svrs s svr)) (t := Commit commit_t v {}))) \<and>
     clock (svrs s' svr) = Suc (max (clock (svrs s svr)) (cl_clock (cls s (get_cl_wtxn t)))) \<and>
     lst (svrs s' svr) =
       (if pending_wtxns s' svr = {} then clock (svrs s svr) else Min (pending_wtxns s' svr)) \<and>
-    cls_svr_k'_t'_unchanged svr s s' \<and>
+    cls_svr_k'_unchanged svr s s' \<and>
     commit_order s' = commit_order s"
 
 subsubsection \<open>The Event System\<close>
@@ -292,7 +302,7 @@ definition state_init :: "'v state" where
                   lst_map = (\<lambda>svr. 0),
                   cl_view = view_txid_init,
                   cl_clock = 0 \<rparr>),
-    svrs = (\<lambda>svr. \<lparr> wtxn_state = Map.empty (T0 \<mapsto> Commit 0 undefined {}),
+    svrs = (\<lambda>svr. \<lparr> wtxn_state = (\<lambda>t. No_Ver) (T0 := Commit 0 undefined {}),
                     clock = 0,
                     lst = 0 \<rparr>),
     commit_order = (\<lambda>k. [T0])
@@ -330,8 +340,8 @@ definition kvs_of_s :: "'v state \<Rightarrow> 'v kv_store" where
   "kvs_of_s s \<equiv>
     (\<lambda>k. map
       (\<lambda>t. case wtxn_state (svrs s k) t of
-        Some (Prep ts v) \<Rightarrow> \<lparr>v_value = v, v_writer = t, v_readerset = {}\<rparr> |
-        Some (Commit cts v rs) \<Rightarrow> \<lparr>v_value = v, v_writer = t, v_readerset = rs\<rparr>)
+        Prep ts v \<Rightarrow> \<lparr>v_value = v, v_writer = t, v_readerset = {}\<rparr> |
+        Commit cts v rs \<Rightarrow> \<lparr>v_value = v, v_writer = t, v_readerset = rs\<rparr>)
       (commit_order s k))"
 
 definition views_of_s :: "'v state \<Rightarrow> (cl_id \<Rightarrow> view)" where
